prove step_map

src/drf/DRF_PF.v
@@ -2032,16 +2032,38 @@ Section MAPPED.
       msg_map (Message.full val released) (Message.full val freleased)
   .
 
+  Inductive memory_op_kind_map (loc: Loc.t) : Memory.op_kind -> Memory.op_kind -> Prop :=
+  | memory_op_kind_map_add
+    :
+      memory_op_kind_map loc (Memory.op_kind_add) (Memory.op_kind_add)
+  | memory_op_kind_map_split
+      to fto msg fmsg
+      (MSG: msg_map msg fmsg)
+      (TO: f loc to fto)
+    :
+      memory_op_kind_map loc (Memory.op_kind_split to msg) (Memory.op_kind_split fto fmsg)
+  | memory_op_kind_map_lower
+      msg fmsg
+      (MSG: msg_map msg fmsg)
+    :
+      memory_op_kind_map loc (Memory.op_kind_lower msg) (Memory.op_kind_lower fmsg)
+  | memory_op_kind_map_cancel
+    :
+      memory_op_kind_map loc (Memory.op_kind_cancel) (Memory.op_kind_cancel)
+  .
+  Hint Constructors memory_op_kind_map.
+
   Inductive tevent_map: ThreadEvent.t -> ThreadEvent.t -> Prop :=
   | tevent_map_promise
-      loc from ffrom to fto msg fmsg kind
+      loc from ffrom to fto msg fmsg kind fkind
       (FROM: f loc from ffrom)
       (TO: f loc to fto)
       (MSG: msg_map msg fmsg)
+      (KIND: memory_op_kind_map loc kind fkind)
     :
       tevent_map
         (ThreadEvent.promise loc from to msg kind)
-        (ThreadEvent.promise loc ffrom fto fmsg kind)
+        (ThreadEvent.promise loc ffrom fto fmsg fkind)
   | tevent_map_read
       loc to fto val released freleased freleased' ordr
       (TO: f loc to fto)
@@ -2055,7 +2077,7 @@ Section MAPPED.
       loc from ffrom to fto val released freleased freleased' ordw
       (FROM: f loc from ffrom)
       (TO: f loc to fto)
-      (RELEASED: opt_view_map released freleased)
+      (RELEASED: opt_view_map released freleased')
       (RELEASEDLE: View.opt_le freleased freleased')
     :
       tevent_map
@@ -2072,7 +2094,7 @@ Section MAPPED.
       (RELEASEDWLE: View.opt_le freleasedw freleasedw')
     :
       tevent_map
-        (ThreadEvent.update loc from to valr valw releasedr releasedr ordr ordw)
+        (ThreadEvent.update loc from to valr valw releasedr releasedw ordr ordw)
         (ThreadEvent.update loc ffrom fto valr valw freleasedr freleasedw ordr ordw)
   | tevent_map_fence
       or ow
@@ -2091,6 +2113,11 @@ Section MAPPED.
       tevent_map
         (ThreadEvent.silent)
         (ThreadEvent.silent)
+  | tevent_map_failure
+    :
+      tevent_map
+        (ThreadEvent.failure)
+        (ThreadEvent.failure)
   .
 
   Definition non_collapsable (loc: Loc.t) (to: Time.t): Prop :=
@@ -3542,27 +3569,6 @@ Section MAPPED.
     i. des. esplits; eauto.
   Qed.
 
-  Inductive memory_op_kind_map (loc: Loc.t) : Memory.op_kind -> Memory.op_kind -> Prop :=
-  | memory_op_kind_map_add
-    :
-      memory_op_kind_map loc (Memory.op_kind_add) (Memory.op_kind_add)
-  | memory_op_kind_map_split
-      to fto msg fmsg
-      (MSG: msg_map msg fmsg)
-      (TO: f loc to fto)
-    :
-      memory_op_kind_map loc (Memory.op_kind_split to msg) (Memory.op_kind_split fto fmsg)
-  | memory_op_kind_map_lower
-      msg fmsg
-      (MSG: msg_map msg fmsg)
-    :
-      memory_op_kind_map loc (Memory.op_kind_lower msg) (Memory.op_kind_lower fmsg)
-  | memory_op_kind_map_cancel
-    :
-      memory_op_kind_map loc (Memory.op_kind_cancel) (Memory.op_kind_cancel)
-  .
-  Hint Constructors memory_op_kind_map.
-
   Lemma promise_map mem0 fmem0 prom0 fprom0 loc from ffrom to fto msg fmsg mem1 prom1 kind
         (MLE: Memory.le fprom0 fmem0)
         (PROMISE: Memory.promise prom0 mem0 loc from to msg prom1 mem1 kind)
@@ -3942,7 +3948,7 @@ Section MAPPED.
     end.
 
   Definition mappable_memory mem :=
-    forall loc to msg (GET: Memory.get loc to mem = Some msg),
+    forall loc to from val released (GET: Memory.get loc to mem = Some (from, Message.full val released)),
       mappable_time loc to.
 
   Lemma mappable_memory_op mem0 loc from to msg mem1 kind
@@ -3953,7 +3959,7 @@ Section MAPPED.
     :
       mappable_memory mem1.
   Proof.
-    ii. destruct msg0 as [from0 msg0]. inv OP.
+    ii. inv OP.
     - erewrite Memory.add_o in GET; eauto. des_ifs; eauto.
       ss. des; clarify.
     - erewrite Memory.split_o in GET; eauto. des_ifs; eauto.
@@ -3971,19 +3977,8 @@ Section MAPPED.
       mappable_memory mem.
   Proof.
     inv MEM. ii.
-    ii.
-
-    econs.
-    ii. destruct msg0 as [from0 msg0]. inv OP.
-    - erewrite Memory.add_o in GET; eauto. des_ifs; eauto.
-      ss. des; clarify.
-    - erewrite Memory.split_o in GET; eauto. des_ifs; eauto.
-      + ss. des; clarify.
-      + ss. des; clarify.
-        eapply Memory.split_get0 in SPLIT. des. eauto.
-    - erewrite Memory.lower_o in GET; eauto. des_ifs; eauto.
-      ss. des; clarify.
-    - erewrite Memory.remove_o in GET; eauto. des_ifs; eauto.
+    eapply MAPPED in GET. des; clarify.
+    eexists. eauto.
   Qed.
 
   Lemma mappable_memory_closed_timemap_exists
@@ -4078,6 +4073,29 @@ Section MAPPED.
       esplits; eauto. econs; eauto.
   Qed.
 
+  Lemma closed_message_map mem fmem msg fmsg
+        (MEM: memory_map mem fmem)
+        (MSG: msg_map msg fmsg)
+        (CLOSED: Memory.closed_message msg mem)
+    :
+      Memory.closed_message fmsg fmem.
+  Proof.
+    inv CLOSED.
+    - inv MSG. econs.
+      eapply closed_opt_view_map; eauto.
+    - inv MSG. econs.
+  Qed.
+
+  Lemma promise_consistent_mon vw0 vw1 prom0 prom1
+        (CONSISTENT: Local.promise_consistent (Local.mk vw1 prom1))
+        (VIEW: TView.le vw0 vw1)
+        (MLE: Memory.le prom0 prom1)
+    :
+      Local.promise_consistent (Local.mk vw0 prom0).
+  Proof.
+    ii. eapply MLE in PROMISE. eapply CONSISTENT in PROMISE.
+    eapply TimeFacts.le_lt_lt; eauto. inv VIEW. inv CUR. ss.
+  Qed.
 
   Lemma step_map
         P lang th0 th1 fth0 st0 st1 lc0 lc1 flc0
@@ -4089,912 +4107,80 @@ Section MAPPED.
         (TH_TGT1: th1 = Thread.mk lang st1 lc1 sc1 mem1)
         (TH_SRC: fth0 = Thread.mk lang st0 flc0 fsc0 fmem0)
         (LCWF: Local.wf flc0 fmem0)
-
+        (CLOSED: Memory.closed fmem0)
         (LOCAL: local_map lc0 flc0)
         (MEM: memory_map mem0 fmem0)
         (SC: timemap_map sc0 fsc0')
         (SCLE: TimeMap.le fsc0 fsc0')
     :
       exists flc1 fmem1 fsc1 fsc1' fe,
+        (<<EVT: tevent_map e fe>>) /\
         (<<STEP: Thread.step_allpf
                    fe fth0
                    (Thread.mk lang st1 flc1 fsc1 fmem1)>>) /\
         (<<SC: timemap_map sc1 fsc1'>>) /\
         (<<SCLE: TimeMap.le fsc1 fsc1'>>) /\
         (<<MEM: memory_map mem1 fmem1>>) /\
-        (<<LOCAL: local_map lc1 flc1>>) /\
-        (<<EVT: tevent_map e fe>>)
+        (<<LOCAL: local_map lc1 flc1>>)
   .
   Proof.
     clarify. inv STEP. eapply MAPPABLE in SAT. inv STEP0. inv STEP.
     - inv STEP0. ss. inv LOCAL. inv LOCAL0. inv LCWF. des.
       exploit mappable_memory_closed_msg_exists; eauto.
-      { eapply mappable_memory_op; eauto.
-
-
-      des. unfold mappable_time in FROM, TO. des.
-      exploit promise_map; eauto.
-      {
-
-
-  Lemma step_map
-        P lang th0 th1 fth st0 st1 vw0 fvw0 vw1 prom0 prom1 fprom0
-        sc0 sc1 fsc0 mem0 mem1 fmem0 e
-        (MAPPABLE: P <1= wf_mappable_evt)
-        (* (PRED: P <1= promise_free) *)
-        (STEP: (@pred_step P lang) e th0 th1)
-        (TH_TGT0: th0 = Thread.mk lang st0 lc0 sc0 mem0)
-        (TH_TGT1: th1 = Thread.mk lang st1 lc1 mem1)
-        (TH_SRC: fth0 = Thread.mk lang st (Local.mk fvw0 prom_src)
-                                 sc_src mem_src)
-
-        (CLOSEDMAP0: Memory.closed_timemap sc_tgt mem_tgt)
-        (CLOSED0: Memory.closed mem_tgt)
-        (LCWF: Local.wf (Local.mk v_tgt prom_tgt) mem_tgt)
-        (INHABITED: Memory.inhabited mem_tgt)
-
-        (TVIEW: tview_map v_src v_tgt)
-        (MEM: memory_map mem_src mem_tgt)
-        (PROM: promises_map prom_src prom_tgt)
-        (SC: timemap_map sc_src sc_tgt)
-    :
-      exists e_src prom_src' v_src' sc_src' mem_src',
-        (<<STEP: Thread.step_allpf
-                   e_src th_src
-                   (Thread.mk lang st' (Local.mk v_src' prom_src') sc_src' mem_src')>>) /\
-        (<<SC: timemap_map sc_src' sc_tgt'>>) /\
-        (<<PROM: promises_map prom_src' prom_tgt'>>) /\
-        (<<MEM: memory_map mem_src' mem_tgt'>>) /\
-        (<<TVIEW: tview_map v_src' v_tgt'>>) /\
-        (<<EVT: tevent_map e_src e_tgt>>)
-  .
-  Proof.
-    clarify. inv STEP. eapply MAPPABLE in SAT. inv STEP0. inv STEP.
-    - inv STEP0. ss. inv LOCAL. ss. clarify.
-      inv LCWF. exploit promise_map.
-      {
-
-
-  Lemma step_map
-        P lang th_src th_tgt th_tgt' st st' v_src v_tgt v_tgt' prom_src prom_tgt prom_tgt'
-        sc_src sc_tgt sc_tgt'
-        mem_src mem_tgt mem_tgt' e_tgt
-        (MAPPABLE: P <1= wf_mappable_evt)
-        (* (PRED: P <1= promise_free) *)
-        (STEP: (@pred_step P lang) e_tgt th_tgt th_tgt')
-        (TH_SRC: th_src = Thread.mk lang st (Local.mk v_src prom_src)
-                                    sc_src mem_src)
-        (TH_TGT0: th_tgt = Thread.mk lang st (Local.mk v_tgt prom_tgt)
-                                     sc_tgt mem_tgt)
-        (TH_TGT1: th_tgt' = Thread.mk lang st' (Local.mk v_tgt' prom_tgt')
-                                      sc_tgt' mem_tgt')
-
-        (CLOSEDMAP0: Memory.closed_timemap sc_tgt mem_tgt)
-        (CLOSED0: Memory.closed mem_tgt)
-        (LCWF: Local.wf (Local.mk v_tgt prom_tgt) mem_tgt)
-        (INHABITED: Memory.inhabited mem_tgt)
-
-        (TVIEW: tview_map v_src v_tgt)
-        (MEM: memory_map mem_src mem_tgt)
-        (PROM: promises_map prom_src prom_tgt)
-        (SC: timemap_map sc_src sc_tgt)
-    :
-      exists e_src prom_src' v_src' sc_src' mem_src',
-        (<<STEP: Thread.step_allpf
-                   e_src th_src
-                   (Thread.mk lang st' (Local.mk v_src' prom_src') sc_src' mem_src')>>) /\
-        (<<SC: timemap_map sc_src' sc_tgt'>>) /\
-        (<<PROM: promises_map prom_src' prom_tgt'>>) /\
-        (<<MEM: memory_map mem_src' mem_tgt'>>) /\
-        (<<TVIEW: tview_map v_src' v_tgt'>>) /\
-        (<<EVT: tevent_map e_src e_tgt>>)
-  .
-  Proof.
-    clarify. inv STEP. eapply MAPPABLE in SAT. inv STEP0. inv STEP.
-    - inv STEP0. ss. inv LOCAL. ss. clarify.
-      inv LCWF. exploit promise_map.
-      {
-
-      promise_map
-
-  Admitted.
-
-
-  (* Lemma step_map *)
-  (*       P lang th_src th_tgt th_tgt' st st' v_src v_tgt v_tgt' prom_src prom_tgt prom_tgt' *)
-  (*       sc_src sc_tgt sc_tgt' *)
-  (*       mem_src mem_tgt mem_tgt' e_tgt *)
-  (*       (MAPPABLE: P <1= wf_mappable_evt) *)
-  (*       (* (PRED: P <1= promise_free) *) *)
-  (*       (STEP: (@pred_step P lang) e_tgt th_tgt th_tgt') *)
-  (*       (TH_SRC: th_src = Thread.mk lang st (Local.mk v_src prom_src) *)
-  (*                                   sc_src mem_src) *)
-  (*       (TH_TGT0: th_tgt = Thread.mk lang st (Local.mk v_tgt prom_tgt) *)
-  (*                                    sc_tgt mem_tgt) *)
-  (*       (TH_TGT1: th_tgt' = Thread.mk lang st' (Local.mk v_tgt' prom_tgt') *)
-  (*                                     sc_tgt' mem_tgt') *)
-
-  (*       (CLOSEDMAP0: Memory.closed_timemap sc_tgt mem_tgt) *)
-  (*       (CLOSED0: Memory.closed mem_tgt) *)
-  (*       (LCWF: Local.wf (Local.mk v_tgt prom_tgt) mem_tgt) *)
-  (*       (INHABITED: Memory.inhabited mem_tgt) *)
-
-  (*       (TVIEW: tview_map v_src v_tgt) *)
-  (*       (MEM: memory_map mem_src mem_tgt) *)
-  (*       (PROM: promises_map prom_src prom_tgt) *)
-  (*       (SC: timemap_map sc_src sc_tgt) *)
-  (*   : *)
-  (*     exists e_src prom_src' v_src' sc_src' mem_src', *)
-  (*       (<<STEP: Thread.step_allpf *)
-  (*                  e_src th_src *)
-  (*                  (Thread.mk lang st' (Local.mk v_src' prom_src') sc_src' mem_src')>>) /\ *)
-  (*       (<<SC: timemap_map sc_src' sc_tgt'>>) /\ *)
-  (*       (<<PROM: promises_map prom_src' prom_tgt'>>) /\ *)
-  (*       (<<MEM: memory_map mem_src' mem_tgt'>>) /\ *)
-  (*       (<<TVIEW: tview_map v_src' v_tgt'>>) /\ *)
-  (*       (<<EVT: tevent_map e_src e_tgt>>) *)
-  (* . *)
-  (* Proof. *)
-  (* Admitted. *)
-
-  (* Lemma remove_memory_map mem0 fmem0 loc from to msg mem1 *)
-  (*       (REMOVE: Memory.remove mem0 loc from to msg mem1) *)
-  (*       (MEM: memory_map mem0 fmem0) *)
-  (*   : *)
-  (*     exists ffrom fto fmsg fmem1, *)
-  (*       (<<TO: f loc to fto>>) /\ *)
-  (*       (<<FROM: f loc from ffrom>>) /\ *)
-  (*       (<<MSG: msg_map msg fmsg>>) /\ *)
-  (*       (<<MEM: promises_map mem1 fmem1>>) /\ *)
-  (*       (<<REMOVE: Memory.remove fmem0 loc ffrom fto fmsg fmem1>>). *)
-  (* Proof. *)
-  (*   exploit Memory.remove_get0; eauto. i. des. *)
-  (*   eapply msg_get_promises_map in GET; eauto. des. *)
-  (*   hexploit (@Memory.remove_exists fmem0 loc ffrom fto fmsg); eauto. *)
-  (*   i. des. esplits; eauto. *)
-  (*   econs. *)
-  (*   - i. erewrite Memory.remove_o in GET1; eauto. des_ifs. ss. *)
-  (*     dup GET1. eapply msg_get_promises_map in GET1; eauto. *)
-  (*     guardH o. des. unguard. *)
-  (*     exists fto0, ffrom0, fmsg0. esplits; eauto. *)
-  (*     erewrite Memory.remove_o; eauto. des_ifs; ss. des; clarify. *)
-  (*     exploit UNIQUE; eauto. i. clarify. *)
-  (*   - i. erewrite Memory.remove_o in GET1; eauto. des_ifs. *)
-  (*     dup MEM. inv MEM. eapply ONLY in GET1. *)
-  (*     guardH o. des. *)
-  (*     esplits; eauto. *)
-  (*     erewrite Memory.remove_o; eauto. *)
-  (*     unguard. ss. des_ifs; ss; eauto. *)
-  (*     des; clarify. exfalso. *)
-  (*     hexploit (map_eq TO0 TO). i. clarify. *)
-  (* Qed. *)
-
-
-
-  (* Definition respecting_memory (P: Loc.t -> Time.t -> Prop) (m: Memory.t) := *)
-  (*   forall loc to from msg (GET: Memory.get loc to m = Some (from, msg)), *)
-  (*     (<<FROM: P loc from>>) /\ (<<TO: P loc to>>). *)
-
-  (* (* Definition respecting_map (P: Loc.t -> Time.t -> Prop) (tm: TimeMap.t) := *) *)
-  (* (*   forall loc, P loc (tm loc). *) *)
-  (* Notation respecting_map P tm := (forall loc, P loc (tm loc)). *)
-
-  (* Inductive respecting_view P view: Prop := *)
-  (* | respecting_view_intro *)
-  (*     (PLN: respecting_map P (View.pln view)) *)
-  (*     (RLX: respecting_map P (View.rlx view)) *)
-  (* . *)
-
-  (* Inductive respecting_opt_view P: option View.t -> Prop := *)
-  (* | respecting_opt_view_some *)
-  (*     vw *)
-  (*     (SOME: respecting_view P vw) *)
-  (*   : *)
-  (*     respecting_opt_view P (Some vw) *)
-  (* | respecting_opt_view_none *)
-  (*   : *)
-  (*     respecting_opt_view P None *)
-  (* . *)
-
-  (* Inductive respecting_tview P tview: Prop := *)
-  (* | respectin_tview_intro *)
-  (*     (REL: forall loc : positive, respecting_view P (TView.rel tview loc)) *)
-  (*     (CUR: respecting_view P (TView.cur tview)) *)
-  (*     (ACQ: respecting_view P (TView.acq tview)) *)
-  (* . *)
-
-  (* Lemma closed_timemap_respecting P m f tm *)
-  (*       (RESPECT: respecting_memory P m) *)
-  (*       (PRSV: prsv P f) *)
-  (*       (CLOSED: Memory.closed_timemap tm m) *)
-  (*   : *)
-  (*     respecting_map P tm. *)
-  (* Proof. *)
-  (*   ii. specialize (CLOSED loc). des. *)
-  (*   eapply RESPECT in CLOSED. des. eauto. *)
-  (* Qed. *)
-
-  (* Lemma closed_view_respecting P m f vw *)
-  (*       (RESPECT: respecting_memory P m) *)
-  (*       (PRSV: prsv P f) *)
-  (*       (CLOSED: Memory.closed_view vw m) *)
-  (*   : *)
-  (*     respecting_view P vw. *)
-  (* Proof. *)
-  (*   inv CLOSED. econs. *)
-  (*   - eapply closed_timemap_respecting; eauto. *)
-  (*   - eapply closed_timemap_respecting; eauto. *)
-  (* Qed. *)
-
-  (* Lemma closed_opt_view_respecting P m f vw *)
-  (*       (RESPECT: respecting_memory P m) *)
-  (*       (PRSV: prsv P f) *)
-  (*       (CLOSED: Memory.closed_opt_view vw m) *)
-  (*   : *)
-  (*     respecting_opt_view P vw. *)
-  (* Proof. *)
-  (*   inv CLOSED. *)
-  (*   - econs. eapply closed_view_respecting; eauto. *)
-  (*   - econs. *)
-  (* Qed. *)
-
-  (* Lemma closed_tview_respecting P m f tvw *)
-  (*       (RESPECT: respecting_memory P m) *)
-  (*       (PRSV: prsv P f) *)
-  (*       (CLOSED: TView.closed tvw m) *)
-  (*   : *)
-  (*     respecting_tview P tvw. *)
-  (* Proof. *)
-  (*   inv CLOSED. econs. *)
-  (*   - i. eapply closed_view_respecting; eauto. *)
-  (*   - eapply closed_view_respecting; eauto. *)
-  (*   - eapply closed_view_respecting; eauto. *)
-  (* Qed. *)
-
-  (* Definition memory_to (m: Memory.t) (l: Loc.t) (t: Time.t): Prop := *)
-  (*   exists from val released, *)
-  (*     (<<GET: Memory.get l t m = Some (from, Message.full val released)>>) *)
-  (* . *)
-
-  (* Lemma memory_to_respecting P m loc to *)
-  (*       (INMEMORY: respecting_memory P m) *)
-  (*       (MEMORYTO: memory_to m loc to) *)
-  (*   : *)
-  (*     P loc to. *)
-  (* Proof. *)
-  (*   unfold memory_to in *. des. *)
-  (*   eapply INMEMORY in GET. des. auto. *)
-  (* Qed. *)
-
-  (* Lemma map_timemap_join P f tm0 tm1 *)
-  (*       (PRSV: prsv P f) *)
-  (*       (CLOSED0: respecting_map P tm0) *)
-  (*       (CLOSED1: respecting_map P tm1) *)
-  (*   : *)
-  (*     timemap_map f (TimeMap.join tm0 tm1) = TimeMap.join (timemap_map f tm0) (timemap_map f tm1). *)
-  (* Proof. *)
-  (*   extensionality t. unfold timemap_map, TimeMap.join. *)
-  (*   eapply map_time_join; eauto. *)
-  (* Qed. *)
-
-  (* Lemma map_viewjoin P f v0 v1 *)
-  (*       (PRSV: prsv P f) *)
-  (*       (CLOSED0: respecting_view P v0) *)
-  (*       (CLOSED1: respecting_view P v1) *)
-  (*   : *)
-  (*     view_map f (View.join v0 v1) = View.join (view_map f v0) (view_map f v1). *)
-  (* Proof. *)
-  (*   inv CLOSED0. inv CLOSED1. *)
-  (*   unfold view_map, View.join. ss. f_equal. *)
-  (*   - eapply map_timemap_join; eauto. *)
-  (*   - eapply map_timemap_join; eauto. *)
-  (* Qed. *)
-
-  (* Lemma map_tviewjoin P f tv0 tv1 *)
-  (*       (PRSV: prsv P f) *)
-  (*       (CLOSED0: respecting_tview P tv0) *)
-  (*       (CLOSED1: respecting_tview P tv1) *)
-  (*   : *)
-  (*     tview_map f (TView.join tv0 tv1) = TView.join (tview_map f tv0) (tview_map f tv1). *)
-  (* Proof. *)
-  (*   inv CLOSED0. inv CLOSED1. *)
-  (*   unfold tview_map, TView.join. ss. f_equal. *)
-  (*   - extensionality l. eapply map_viewjoin; eauto. *)
-  (*   - eapply map_viewjoin; eauto. *)
-  (*   - eapply map_viewjoin; eauto. *)
-  (* Qed. *)
-
-  (* Lemma map_unwrap P f released *)
-  (*       (PRSV: prsv P f) *)
-  (*       (CLOSED0: respecting_opt_view P released) *)
-  (*   : *)
-  (*     view_map f (View.unwrap released) = *)
-  (*     View.unwrap (option_map (view_map f) released). *)
-  (* Proof. *)
-  (*   unfold View.unwrap. des_ifs. eapply map_view_bot; eauto. *)
-  (* Qed. *)
-
-  (* Lemma map_read_tview P f m v loc to released ord *)
-  (*       (PRSV: prsv P f) *)
-  (*       (INMEMORY: respecting_memory P m) *)
-  (*       (CLOSED0: TView.closed v m) *)
-  (*       (CLOSED1: Memory.closed_opt_view released m) *)
-  (*       (CLOSED2: memory_to m loc to) *)
-  (*       (INHABITED: Memory.inhabited m) *)
-  (*   : *)
-  (*     tview_map f (TView.read_tview v loc to released ord) = *)
-  (*     TView.read_tview (tview_map f v) loc (f loc to) (option_map (view_map f) released) ord. *)
-  (* Proof. *)
-  (*   dup CLOSED0. dup CLOSED1. dup CLOSED0. *)
-  (*   eapply closed_tview_respecting in CLOSED0; eauto. *)
-  (*   eapply closed_opt_view_respecting in CLOSED1; eauto. *)
-  (*   eapply memory_to_respecting in CLOSED2; eauto. *)
-  (*   unfold tview_map, TView.read_tview. ss. *)
-  (*   repeat (erewrite <- map_unwrap; eauto). *)
-  (*   repeat (erewrite map_viewjoin; eauto). *)
-  (*   - erewrite map_singleton_ur_if; eauto. *)
-  (*     des_ifs; f_equal; erewrite map_view_bot; eauto. *)
-  (*   - inv CLOSED0. auto. *)
-  (*   - eapply *)
-
-  (*     unfold times_in_memory_to in *. des. *)
-  (*     eapply Memory.singleton_ur_if_closed_view; eauto. *)
-  (*   - eapply Memory.join_closed_view; eauto. *)
-  (*     + inv CLOSED0; eauto. *)
-  (*     + unfold times_in_memory_to in *. des. *)
-  (*       eapply Memory.singleton_ur_if_closed_view; eauto. *)
-  (*   - des_ifs. *)
-  (*     + eapply Memory.unwrap_closed_opt_view; eauto. *)
-  (*     + eapply Memory.closed_view_bot; eauto. *)
-  (*   - inv CLOSED0. eauto. *)
-  (*   - unfold times_in_memory_to in *. des. *)
-  (*     eapply Memory.singleton_ur_if_closed_view; eauto. *)
-  (*   - eapply Memory.join_closed_view; eauto. *)
-  (*     + inv CLOSED0; eauto. *)
-  (*     + unfold times_in_memory_to in *. des. *)
-  (*       eapply Memory.singleton_ur_if_closed_view; eauto. *)
-  (*   - des_ifs. *)
-  (*     + eapply Memory.unwrap_closed_opt_view; eauto. *)
-  (*     + eapply Memory.closed_view_bot; eauto. *)
-  (* Qed. *)
-
-
-  (* Definition times_in_memory (m: Memory.t) (l: Loc.t) (t: Time.t): Prop := *)
-  (*   (<<OFFROM: exists to msg, *)
-  (*       (<<GET: Memory.get l to m = Some (t, msg)>>)>>) \/ *)
-  (*   (<<OFTO: exists from msg, *)
-  (*       (<<GET: Memory.get l t m = Some (from, msg)>>)>>) *)
-  (* . *)
-
-  (* Definition times_in_memory_to (m: Memory.t) (l: Loc.t) (t: Time.t): Prop := *)
-  (*   (<<OFTO: exists from val released, *)
-  (*       (<<GET: Memory.get l t m = Some (from, Message.full val released)>>)>>) *)
-  (* . *)
-
-  (* Lemma times_in_memory_to_in_memory: *)
-  (*   times_in_memory_to <3= times_in_memory. *)
-  (* Proof. *)
-  (*   i. unfold times_in_memory_to in *. des. right. eauto. *)
-  (* Qed. *)
-  (* Hint Resolve times_in_memory_to_in_memory. *)
-
-  (* Lemma map_closed_timemap m f tm *)
-  (*       (INMEMORY: map_preserving (times_in_memory m) f) *)
-  (*       (CLOSED: Memory.closed_timemap tm m) *)
-  (*   : *)
-  (*     forall loc, times_in_memory m loc (tm loc). *)
-  (* Proof. *)
-  (*   ii. right. specialize (CLOSED loc). unfold times_in_memory_to. des. eauto. *)
-  (* Qed. *)
-
-  (* Lemma map_timemap_join f m tm0 tm1 *)
-  (*       (INMEMORY: map_preserving (times_in_memory m) f) *)
-  (*       (CLOSED0: Memory.closed_timemap tm0 m) *)
-  (*       (CLOSED1: Memory.closed_timemap tm1 m) *)
-  (*   : *)
-  (*     timemap_map f (TimeMap.join tm0 tm1) = TimeMap.join (timemap_map f tm0) (timemap_map f tm1). *)
-  (* Proof. *)
-  (*   extensionality t. unfold timemap_map, TimeMap.join. *)
-  (*   eapply map_time_join; eauto. *)
-  (*   - eapply map_closed_timemap; eauto. *)
-  (*   - eapply map_closed_timemap; eauto. *)
-  (* Qed. *)
-
-  (* Lemma map_viewjoin f m v0 v1 *)
-  (*       (INMEMORY: map_preserving (times_in_memory m) f) *)
-  (*       (CLOSED0: Memory.closed_view v0 m) *)
-  (*       (CLOSED1: Memory.closed_view v1 m) *)
-  (*   : *)
-  (*     view_map f (View.join v0 v1) = View.join (view_map f v0) (view_map f v1). *)
-  (* Proof. *)
-  (*   inv CLOSED0. inv CLOSED1. *)
-  (*   unfold view_map, View.join. ss. f_equal. *)
-  (*   - eapply map_timemap_join; eauto. *)
-  (*   - eapply map_timemap_join; eauto. *)
-  (* Qed. *)
-
-  (* Lemma map_tviewjoin f m tv0 tv1 *)
-  (*       (INMEMORY: map_preserving (times_in_memory m) f) *)
-  (*       (CLOSED0: TView.closed tv0 m) *)
-  (*       (CLOSED1: TView.closed tv1 m) *)
-  (*   : *)
-  (*     tview_map f (TView.join tv0 tv1) = TView.join (tview_map f tv0) (tview_map f tv1). *)
-  (* Proof. *)
-  (*   inv CLOSED0. inv CLOSED1. *)
-  (*   unfold tview_map, TView.join. ss. f_equal. *)
-  (*   - extensionality l. eapply map_viewjoin; eauto. *)
-  (*   - eapply map_viewjoin; eauto. *)
-  (*   - eapply map_viewjoin; eauto. *)
-  (* Qed. *)
-
-  (* Lemma map_unwrap f m released *)
-  (*       (INMEMORY: map_preserving (times_in_memory m) f) *)
-  (*       (CLOSED0: Memory.closed_opt_view released m) *)
-  (*   : *)
-  (*     view_map f (View.unwrap released) = *)
-  (*     View.unwrap (option_map (view_map f) released). *)
-  (* Proof. *)
-  (*   unfold View.unwrap. des_ifs. eapply map_view_bot; eauto. *)
-  (* Qed. *)
-
-  (* Lemma map_read_tview f m v loc to released ord *)
-  (*       (INMEMORY: map_preserving (times_in_memory m) f) *)
-  (*       (CLOSED0: TView.closed v m) *)
-  (*       (CLOSED1: Memory.closed_opt_view released m) *)
-  (*       (CLOSED2: times_in_memory_to m loc to) *)
-  (*       (INHABITED: Memory.inhabited m) *)
-  (*   : *)
-  (*     tview_map f (TView.read_tview v loc to released ord) = *)
-  (*     TView.read_tview (tview_map f v) loc (f loc to) (option_map (view_map f) released) ord. *)
-  (* Proof. *)
-  (*   unfold tview_map, TView.read_tview. ss. *)
-  (*   repeat (erewrite <- map_unwrap; eauto). *)
-  (*   repeat (erewrite map_viewjoin; eauto). *)
-  (*   - erewrite map_singleton_ur_if; eauto. *)
-  (*     des_ifs; f_equal; erewrite map_view_bot; eauto. *)
-  (*   - inv CLOSED0. eauto. *)
-  (*   - unfold times_in_memory_to in *. des. *)
-  (*     eapply Memory.singleton_ur_if_closed_view; eauto. *)
-  (*   - eapply Memory.join_closed_view; eauto. *)
-  (*     + inv CLOSED0; eauto. *)
-  (*     + unfold times_in_memory_to in *. des. *)
-  (*       eapply Memory.singleton_ur_if_closed_view; eauto. *)
-  (*   - des_ifs. *)
-  (*     + eapply Memory.unwrap_closed_opt_view; eauto. *)
-  (*     + eapply Memory.closed_view_bot; eauto. *)
-  (*   - inv CLOSED0. eauto. *)
-  (*   - unfold times_in_memory_to in *. des. *)
-  (*     eapply Memory.singleton_ur_if_closed_view; eauto. *)
-  (*   - eapply Memory.join_closed_view; eauto. *)
-  (*     + inv CLOSED0; eauto. *)
-  (*     + unfold times_in_memory_to in *. des. *)
-  (*       eapply Memory.singleton_ur_if_closed_view; eauto. *)
-  (*   - des_ifs. *)
-  (*     + eapply Memory.unwrap_closed_opt_view; eauto. *)
-  (*     + eapply Memory.closed_view_bot; eauto. *)
-  (* Qed. *)
-
-  (* Lemma map_step_read *)
-  (*       f v v' prom_src prom_tgt prom_tgt' *)
-  (*       mem_src mem_tgt loc to val released ord *)
-  (*       (STEP: Local.read_step (Local.mk v prom_tgt) mem_tgt loc to val released ord *)
-  (*                              (Local.mk v' prom_tgt')) *)
-  (*       (INMEMORY0: map_preserving (times_in_memory mem_tgt) f) *)
-  (*       (CLOSED0: Memory.closed mem_tgt) *)
-  (*       (LCWF: Local.wf (Local.mk v Memory.bot) mem_tgt) *)
-  (*       (MEM: memory_map f mem_src mem_tgt) *)
-  (*       (INHABITED: Memory.inhabited mem_tgt) *)
-  (*   : *)
-  (*     (<<STEP: Local.read_step (Local.mk (tview_map f v) prom_src) mem_src loc *)
-  (*                              (f loc to) val (option_map (view_map f) released) ord *)
-  (*                              (Local.mk (tview_map f v') prom_src)>>). *)
-  (* Proof. *)
-  (*   inv STEP. ss. clarify. econs; eauto. *)
-  (*   + inv MEM. exploit MAPPED; eauto. *)
-  (*   + ss. inv READABLE. unfold view_map, option_map, timemap_map. des_ifs. *)
-  (*     * econs; ss; eauto. *)
-  (*       { eapply map_preserving_le_if; eauto. *)
-  (*         - inv LCWF. ss. inv TVIEW_CLOSED. inv CUR. *)
-  (*           eapply map_closed_timemap; eauto. *)
-  (*         - right. eauto. } *)
-  (*       { i. eapply map_preserving_le_if; eauto. *)
-  (*         - inv LCWF. ss. inv TVIEW_CLOSED. inv CUR. *)
-  (*           eapply map_closed_timemap; eauto. *)
-  (*         - right. eauto. } *)
-  (*     * econs; ss; eauto. *)
-  (*       { eapply map_preserving_le_if; eauto. *)
-  (*         - inv LCWF. ss. inv TVIEW_CLOSED. inv CUR. *)
-  (*           eapply map_closed_timemap; eauto. *)
-  (*         - right. eauto. } *)
-  (*       { i. eapply map_preserving_le_if; eauto. *)
-  (*         - inv LCWF. ss. inv TVIEW_CLOSED. inv CUR. *)
-  (*           eapply map_closed_timemap; eauto. *)
-  (*         - right. eauto. } *)
-  (*   + ss. f_equal. erewrite map_read_tview; eauto. *)
-  (*     * inv LCWF. ss. *)
-  (*     * eapply CLOSED0 in GET. des. inv MSG_CLOSED. eauto. *)
-  (*     * unfold times_in_memory_to. eauto. *)
-  (* Qed. *)
-
-  (* Lemma view_map_le f m tm0 tm1 *)
-  (*       (INMEMORY: map_preserving (times_in_memory m) f) *)
-  (*       (CLOSED0: Memory.closed_timemap tm0 m) *)
-  (*       (CLOSED1: Memory.closed_timemap tm1 m) *)
-  (*       (LE: TimeMap.le tm0 tm1) *)
-  (*   : *)
-  (*     TimeMap.le (timemap_map f tm0) (timemap_map f tm1). *)
-  (* Proof. *)
-  (*   ii. unfold timemap_map. *)
-  (*   eapply map_preserving_le_if; eauto. *)
-  (*   - right. specialize (CLOSED0 loc). des. eauto. *)
-  (*   - right. specialize (CLOSED1 loc). des. eauto. *)
-  (* Qed. *)
-
-  (* Lemma view_map_wf f m view *)
-  (*       (INMEMORY: map_preserving (times_in_memory m) f) *)
-  (*       (CLOSED0: Memory.closed_view view m) *)
-  (*       (WF : View.wf view) *)
-  (*   : *)
-  (*     View.wf (view_map f view). *)
-  (* Proof. *)
-  (*   unfold view_map. ss. econs. inv WF. *)
-  (*   inv CLOSED0. eapply view_map_le in PLN_RLX; eauto. *)
-  (* Qed. *)
-
-  (* Lemma map_write_released f m v sc loc to releasedm ord *)
-  (*       (INMEMORY0: map_preserving (times_in_memory m) f) *)
-  (*       (INHABITED: Memory.inhabited m) *)
-  (*       (CLOSED0: Memory.closed m) *)
-  (*       (CLOSED1: Memory.closed_opt_view releasedm m) *)
-  (*       (CLOSED2: times_in_memory_to m loc to) *)
-  (*       (CLOSED3: TView.closed v m) *)
-  (*       (CLOSED4: Memory.closed_timemap sc m) *)
-  (*   : *)
-  (*     option_map (view_map f) (TView.write_released v sc loc to releasedm ord) = *)
-  (*     TView.write_released (tview_map f v) (timemap_map f sc) loc (f loc to) *)
-  (*                          (option_map (view_map f) releasedm) ord. *)
-  (* Proof. *)
-  (*   dup CLOSED2. unfold times_in_memory_to in CLOSED2. des. *)
-  (*   exploit TViewFacts.get_closed_released; eauto. *)
-  (*   instantiate (1:=ord). i. *)
-  (*   unfold TView.write_released in *. des_ifs. unfold option_map. *)
-  (*   erewrite map_viewjoin; eauto. *)
-  (*   - f_equal. erewrite map_unwrap; eauto. f_equal. *)
-  (*     setoid_rewrite LocFun.add_spec_eq. *)
-  (*     des_ifs. *)
-  (*     + erewrite map_viewjoin; eauto. *)
-  (*       * erewrite map_singleton_ur; eauto. *)
-  (*       * inv CLOSED3. eauto. *)
-  (*       * unfold times_in_memory_to in *. des. *)
-  (*         eapply Memory.singleton_ur_closed_view; eauto. *)
-  (*     + erewrite map_viewjoin; eauto. *)
-  (*       * erewrite map_singleton_ur; eauto. *)
-  (*       * inv CLOSED3. eauto. *)
-  (*       * unfold times_in_memory_to in *. des. *)
-  (*         eapply Memory.singleton_ur_closed_view; eauto. *)
-  (*   - eapply Memory.unwrap_closed_opt_view; eauto. *)
-  (*   - exploit TViewFacts.get_closed_tview; eauto. i. *)
-  (*     inv x1. eauto. *)
-  (* Qed. *)
-
-  (* Lemma map_write_tview f m v sc ord loc to *)
-  (*       (INMEMORY: map_preserving (times_in_memory m) f) *)
-  (*       (INHABITED: Memory.inhabited m) *)
-  (*       (CLOSED0: TView.closed v m) *)
-  (*       (CLOSED1: Memory.closed_timemap sc m) *)
-  (*       (CLOSED2: times_in_memory_to m loc to) *)
-  (*   : *)
-  (*     tview_map f (TView.write_tview v sc loc to ord) = *)
-  (*     TView.write_tview (tview_map f v) (timemap_map f sc) loc (f loc to) ord. *)
-  (* Proof. *)
-  (*   unfold TView.write_tview. ss. unfold tview_map at 1. ss. f_equal. *)
-  (*   - extensionality l. des_ifs. *)
-  (*     + setoid_rewrite LocFun.add_spec. des_ifs. *)
-  (*       erewrite map_viewjoin; eauto. *)
-  (*       * f_equal. erewrite map_singleton_ur; eauto. *)
-  (*       * inv CLOSED0. eauto. *)
-  (*       * unfold times_in_memory_to in *. des. *)
-  (*         eapply Memory.singleton_ur_closed_view; eauto. *)
-  (*     + setoid_rewrite LocFun.add_spec. des_ifs. *)
-  (*       erewrite map_viewjoin; eauto. *)
-  (*       * f_equal. erewrite map_singleton_ur; eauto. *)
-  (*       * inv CLOSED0. eauto. *)
-  (*       * unfold times_in_memory_to in *. des. *)
-  (*         eapply Memory.singleton_ur_closed_view; eauto. *)
-  (*   - erewrite map_viewjoin; eauto. *)
-  (*     + f_equal. erewrite map_singleton_ur; eauto. *)
-  (*     + inv CLOSED0. eauto. *)
-  (*     + unfold times_in_memory_to in *. des. *)
-  (*       eapply Memory.singleton_ur_closed_view; eauto. *)
-  (*   - erewrite map_viewjoin; eauto. *)
-  (*     + f_equal. erewrite map_singleton_ur; eauto. *)
-  (*     + inv CLOSED0. eauto. *)
-  (*     + unfold times_in_memory_to in *. des. *)
-  (*       eapply Memory.singleton_ur_closed_view; eauto. *)
-  (* Qed. *)
-
-  (* Lemma map_step_write f v v' prom' *)
-  (*       loc from to val releasedm released ord sc sc' mem_src *)
-  (*       mem_tgt mem_tgt' kind *)
-  (*       (WRITE: Local.write_step *)
-  (*                 (Local.mk v Memory.bot) sc mem_tgt *)
-  (*                 loc from to val releasedm released ord *)
-  (*                 (Local.mk v' prom') sc' mem_tgt' kind) *)
-  (*       (INMEMORY0: map_preserving (times_in_memory mem_tgt) f) *)
-  (*       (INMEMORY1: map_preserving (times_in_memory mem_tgt') f) *)
-  (*       (CLOSED0: Memory.closed mem_tgt) *)
-  (*       (CLOSED1: View.opt_wf releasedm) *)
-  (*       (CLOSED2: Memory.closed_opt_view releasedm mem_tgt) *)
-  (*       (CLOSED3: Memory.closed_timemap sc mem_tgt) *)
-  (*       (LCWF: Local.wf (Local.mk v Memory.bot) mem_tgt) *)
-  (*       (MEM: memory_map f mem_src mem_tgt) *)
-  (*       (INHABITED: Memory.inhabited mem_tgt) *)
-  (*   : *)
-  (*     exists mem_src', *)
-  (*       (<<WRITE: Local.write_step *)
-  (*                   (Local.mk (tview_map f v) Memory.bot) *)
-  (*                   (timemap_map f sc) *)
-  (*                   mem_src loc (f loc from) (f loc to) val *)
-  (*                   (option_map (view_map f) releasedm) *)
-  (*                   (option_map (view_map f) released) ord *)
-  (*                   (Local.mk (tview_map f v') Memory.bot) *)
-  (*                   (timemap_map f sc') mem_src' Memory.op_kind_add>>) /\ *)
-  (*       (<<MEM: memory_map f mem_src' mem_tgt'>>). *)
-  (* Proof. *)
-  (*   inv LCWF. exploit write_msg_wf; eauto. i. des. *)
-  (*   dup WRITE. inv WRITE. ss. clarify. exploit memory_write_bot_add; eauto. i. clarify. *)
-  (*   assert (CLOSEDV1: Memory.closed_opt_view (TView.write_released v sc loc to releasedm ord) mem_tgt'). *)
-  (*   { inv WRITE1. inv PROMISE. ss. *)
-  (*     eapply TViewFacts.write_future; eauto. } *)
-  (*   exploit Local.write_step_future; eauto. i. ss. des. *)
-  (*   inv WRITE1. inv PROMISE. dup MEM0. eapply Memory.add_get0 in MEM1. des. *)
-  (*   exploit write_succeed. *)
-  (*   { instantiate (1:=f loc to). instantiate (1:=f loc from). *)
-  (*     instantiate (1:=mem_src). instantiate (1:=loc). *)
-  (*     ii. inv COVER. *)
-  (*     inv MEM. ss. exploit ONLY; eauto. i. des. clarify. *)
-  (*     destruct msg0. dup GET2. eapply MAPPED in GET2. clarify. *)
-  (*     dup GET3. eapply Memory.add_get1 in GET3; eauto. *)
-  (*     destruct H. destruct ITV. ss. *)
-  (*     assert (LT0: Time.lt (f loc t0) (f loc to)). *)
-  (*     { eapply DenseOrder.DenseOrderFacts.lt_le_lt; eauto. } *)
-  (*     assert (LT1: Time.lt (f loc from) (f loc to1)). *)
-  (*     { eapply DenseOrder.DenseOrderFacts.lt_le_lt; eauto. } *)
-  (*     assert (LT2: Time.lt (f loc from) (f loc to)). *)
-  (*     { eapply DenseOrder.DenseOrderFacts.lt_le_lt; try apply FROM; eauto. } *)
-  (*     assert (LT3: Time.lt (f loc t0) (f loc to1)). *)
-  (*     { eapply DenseOrder.DenseOrderFacts.lt_le_lt; try apply FROM0; eauto. } *)
-  (*     erewrite <- map_preserving_lt_iff in LT0; eauto; cycle 1. *)
-  (*     { left. eauto. } *)
-  (*     { right. eauto. } *)
-  (*     erewrite <- map_preserving_lt_iff in LT1; eauto; cycle 1. *)
-  (*     { left. eauto. } *)
-  (*     { right. eauto. } *)
-  (*     erewrite <- map_preserving_lt_iff in LT2; eauto; cycle 1. *)
-  (*     { left. eauto. } *)
-  (*     { right. eauto. } *)
-  (*     erewrite <- map_preserving_lt_iff in LT3; eauto; cycle 1. *)
-  (*     { left. eauto. } *)
-  (*     { right. eauto. } *)
-  (*     exploit Memory.get_disjoint. *)
-  (*     - eapply GET3. *)
-  (*     - eapply GET0. *)
-  (*     - i. des; clarify. *)
-  (*       exploit Time.middle_spec. *)
-  (*       { instantiate (1:=Time.meet to to1). instantiate (1:=Time.join from t0). *)
-  (*         unfold Time.join, Time.meet. des_ifs. } i. des. *)
-  (*       eapply x0. *)
-  (*       + instantiate (1:=Time.middle (Time.join from t0) (Time.meet to to1)). econs; ss. *)
-  (*         * eapply DenseOrder.DenseOrderFacts.le_lt_lt; eauto. eapply Time.join_r. *)
-  (*         * left. eapply DenseOrder.DenseOrderFacts.lt_le_lt; eauto. eapply Time.meet_r. *)
-  (*       + econs; ss. *)
-  (*         * eapply DenseOrder.DenseOrderFacts.le_lt_lt; eauto. eapply Time.join_l. *)
-  (*         * left. eapply DenseOrder.DenseOrderFacts.lt_le_lt; eauto. eapply Time.meet_l. } *)
-  (*   { instantiate (1:=option_map *)
-  (*                       (view_map f) *)
-  (*                       (TView.write_released v sc loc to releasedm ord)). *)
-  (*     erewrite map_preserving_le_iff in REL_TS; try apply INMEMORY1; eauto. *)
-  (*     - instantiate (1:=loc) in REL_TS. *)
-  (*       setoid_rewrite <- map_unwrap; try apply INMEMORY1; eauto. *)
-  (*     - right. eapply Memory.unwrap_closed_opt_view in CLOSEDV1; eauto. *)
-  (*       + inv CLOSEDV1. specialize (RLX loc). des. eauto. *)
-  (*       + eapply inhabited_future; eauto. *)
-  (*     - right. eauto. } *)
-  (*   { erewrite <- map_preserving_lt_iff; eauto. *)
-  (*     - left. eauto. *)
-  (*     - right. eauto. } *)
-  (*   { econs. inv REL_WF; ss. econs. eapply view_map_wf; try apply INMEMORY1; eauto. *)
-  (*     inv CLOSEDV1; congruence. } *)
-  (*   i. des. exists mem2. esplits; eauto. *)
-  (*   - econs; ss; eauto. *)
-  (*     + erewrite map_write_released; try apply INMEMORY1; eauto. *)
-  (*       * eapply inhabited_future; eauto. *)
-  (*       * eapply Memory.future_closed_opt_view; eauto. *)
-  (*       * unfold times_in_memory_to. eauto. *)
-  (*       * eapply TView.future_closed; eauto. *)
-  (*     + inv WRITABLE. econs. unfold view_map, timemap_map. ss. *)
-  (*       erewrite <- map_preserving_lt_iff; eauto. *)
-  (*       * eapply TView.future_closed in TVIEW_CLOSED; eauto. *)
-  (*         inv TVIEW_CLOSED. inv CUR. specialize (RLX loc). des. *)
-  (*         unfold times_in_memory. eauto. *)
-  (*       * unfold times_in_memory. eauto. *)
-  (*     + f_equal. eapply map_write_tview; eauto. *)
-  (*       * eapply inhabited_future; eauto. *)
-  (*       * eapply TView.future_closed; eauto. *)
-  (*       * unfold times_in_memory_to. eauto. *)
-  (*   - inv WRITE. inv PROMISE. econs. *)
-  (*     + i. erewrite Memory.add_o in GET1; eauto. *)
-  (*       erewrite Memory.add_o; eauto. des_ifs; ss. *)
-  (*       * des; clarify. *)
-  (*       * des; clarify. exfalso. *)
-  (*         erewrite <- map_preserving_eq_iff in a0; eauto. *)
-  (*         { right. eapply Memory.add_get1 in GET1; eauto. } *)
-  (*         { right. eauto. } *)
-  (*       * des; clarify. *)
-  (*       * inv MEM. eauto. *)
-  (*     + i. erewrite Memory.add_o in GET1; eauto. des_ifs. *)
-  (*       * ss; des; clarify. esplits; eauto. *)
-  (*       * inv MEM. exploit ONLY; eauto. i. *)
-  (*         destruct x as [to0 [msg [FROM GET2]]]. *)
-  (*         exists to0, msg. esplits; eauto. *)
-  (*         erewrite Memory.add_o; eauto. des_ifs. *)
-  (*         ss. des; clarify. *)
-  (* Qed. *)
-
-  (* Lemma map_read_fence_tview f v ord *)
-  (*   : *)
-  (*     tview_map f (TView.read_fence_tview v ord) = *)
-  (*     TView.read_fence_tview (tview_map f v) ord. *)
-  (* Proof. *)
-  (*   unfold TView.read_fence_tview, tview_map. ss. f_equal. *)
-  (*   des_ifs. *)
-  (* Qed. *)
-
-  (* Lemma map_write_fence_sc f m v sc ord *)
-  (*       (INMEMORY: map_preserving (times_in_memory m) f) *)
-  (*       (CLOSED0: TView.closed v m) *)
-  (*       (CLOSED1: Memory.closed_timemap sc m) *)
-  (*   : *)
-  (*     timemap_map f (TView.write_fence_sc v sc ord) = *)
-  (*     TView.write_fence_sc (tview_map f v) (timemap_map f sc) ord. *)
-  (* Proof. *)
-  (*   unfold TView.write_fence_sc. ss. *)
-  (*   extensionality loc. des_ifs. *)
-  (*   erewrite map_timemap_join; eauto. *)
-  (*   inv CLOSED0. inv CUR. eauto. *)
-  (* Qed. *)
-
-  (* Lemma map_read_fence f v ord *)
-  (*   : *)
-  (*     tview_map f (TView.read_fence_tview v ord) = *)
-  (*     TView.read_fence_tview (tview_map f v) ord. *)
-  (* Proof. *)
-  (*   unfold TView.read_fence_tview, tview_map. ss. f_equal. des_ifs. *)
-  (* Qed. *)
-
-  (* Lemma write_fence_sc_closed v sc ord m *)
-  (*       (CLOSED0: TView.closed v m) *)
-  (*       (CLOSED1: Memory.closed_timemap sc m) *)
-  (*   : *)
-  (*     Memory.closed_timemap (TView.write_fence_sc v sc ord) m. *)
-  (* Proof. *)
-  (*   unfold TView.write_fence_sc. des_ifs. *)
-  (*   eapply Memory.join_closed_timemap; eauto. *)
-  (*   inv CLOSED0. inv CUR. auto. *)
-  (* Qed. *)
-
-  (* Lemma read_fence_closed tview ord m *)
-  (*       (CLOSED0: TView.closed tview m) *)
-  (*   : *)
-  (*     TView.closed (TView.read_fence_tview tview ord) m. *)
-  (* Proof. *)
-  (*   unfold TView.read_fence_tview. inv CLOSED0. des_ifs. *)
-  (* Qed. *)
-
-  (* Lemma map_write_fence_tview f m v sc ord *)
-  (*       (INMEMORY: map_preserving (times_in_memory m) f) *)
-  (*       (CLOSED0: TView.closed v m) *)
-  (*       (CLOSED1: Memory.closed_timemap sc m) *)
-  (*       (INHABITED: Memory.inhabited m) *)
-  (*   : *)
-  (*     tview_map f (TView.write_fence_tview v sc ord) = *)
-  (*     TView.write_fence_tview (tview_map f v) (timemap_map f sc) ord. *)
-  (* Proof. *)
-  (*   unfold TView.write_fence_tview. ss. *)
-  (*   erewrite <- map_write_fence_sc; eauto. *)
-  (*   unfold tview_map at 1. ss. f_equal. *)
-  (*   - extensionality loc. des_ifs. *)
-  (*   - des_ifs. *)
-  (*   - erewrite map_viewjoin; eauto. *)
-  (*     + des_ifs. erewrite map_view_bot; eauto. *)
-  (*     + inv CLOSED0. inv ACQ. auto. *)
-  (*     + des_ifs. *)
-  (*       * econs; ss; eapply write_fence_sc_closed; eauto. *)
-  (*       * eapply Memory.closed_view_bot; eauto. *)
-  (* Qed. *)
-
-  (* Lemma times_in_memory_le mem0 mem1 *)
-  (*       (MLE: Memory.le mem0 mem1) *)
-  (*   : *)
-  (*     times_in_memory mem0 <2= times_in_memory mem1. *)
-  (* Proof. *)
-  (*   ii. inv PR. *)
-  (*   - des. left. esplits; eauto. *)
-  (*   - des. right. esplits; eauto. *)
-  (* Qed. *)
-
-  (* Lemma map_preserving_memory_le f mem0 mem1 *)
-  (*       (PRSV: map_preserving (times_in_memory mem1) f) *)
-  (*       (MLE: Memory.le mem0 mem1) *)
-  (*   : *)
-  (*     map_preserving (times_in_memory mem0) f. *)
-  (* Proof. *)
-  (*   inv PRSV. econs; eauto. *)
-  (*   i. eapply PRSVLT; eauto. *)
-  (*   - eapply times_in_memory_le; eauto. *)
-  (*   - eapply times_in_memory_le; eauto. *)
-  (* Qed. *)
-
-  (* Lemma map_step *)
-  (*       f lang th_src th_tgt th_tgt' st st' v v' prom' sc sc' *)
-  (*       mem_src mem_tgt mem_tgt' e_tgt *)
-  (*       (STEP: (@pred_step no_promise lang) e_tgt th_tgt th_tgt') *)
-  (*       (TH_SRC: th_src = Thread.mk lang st (Local.mk (tview_map f v) Memory.bot) *)
-  (*                                   (timemap_map f sc) mem_src) *)
-  (*       (TH_TGT0: th_tgt = Thread.mk lang st (Local.mk v Memory.bot) sc mem_tgt) *)
-  (*       (TH_TGT1: th_tgt' = Thread.mk lang st' (Local.mk v' prom') sc' mem_tgt') *)
-  (*       (INMEMORY1: map_preserving (times_in_memory mem_tgt') f) *)
-  (*       (CLOSEDMAP0: Memory.closed_timemap sc mem_tgt) *)
-  (*       (CLOSED0: Memory.closed mem_tgt) *)
-  (*       (LCWF: Local.wf (Local.mk v Memory.bot) mem_tgt) *)
-  (*       (INHABITED: Memory.inhabited mem_tgt) *)
-  (*       (MEM: memory_map f mem_src mem_tgt) *)
-  (*   : *)
-  (*     exists mem_src', *)
-  (*       (<<STEP: (@pred_step no_promise lang) *)
-  (*                  (tevent_map f e_tgt) th_src *)
-  (*                  (Thread.mk lang st' (Local.mk (tview_map f v') Memory.bot) (timemap_map f sc') mem_src')>>) /\ *)
-  (*       (<<MEM: memory_map f mem_src' mem_tgt'>>). *)
-  (* Proof. *)
-  (*   assert (INMEMORY0: map_preserving (times_in_memory mem_tgt) f). *)
-  (*   { eapply map_preserving_memory_le; eauto. clarify. *)
-  (*     hexploit pf_step_memory_le; eauto. } *)
-  (*   clarify. inv STEP. inv STEP0. inv STEP; inv STEP0; ss. inv LOCAL; ss. *)
-  (*   - exists mem_src. esplits; ss; eauto. *)
-  (*     econs; eauto. econs; eauto. econs 2; eauto. econs; eauto. *)
-  (*   - exploit map_step_read; eauto. i. des. *)
-  (*     exists mem_src. esplits; eauto. econs; eauto. econs; eauto. *)
-  (*     econs 2; eauto. econs; eauto. *)
-  (*   - exploit map_step_write; eauto. i. des. ss. *)
-  (*     exists mem_src'. esplits; eauto. econs; eauto. econs; eauto. *)
-  (*     econs 2; eauto. econs; eauto. *)
-  (*   - exploit Local.read_step_future; eauto. i. des. *)
-  (*     destruct lc2. exploit map_step_read; eauto. i. des. *)
-  (*     inv LOCAL1. ss. clarify. *)
-  (*     exploit map_step_write; eauto. i. des. *)
-  (*     exists mem_src'. esplits; eauto. econs; eauto. econs; eauto. *)
-  (*     econs 2; eauto. econs; eauto. *)
-  (*   - exists mem_src. esplits; eauto. econs; eauto. econs; eauto. *)
-  (*     econs 2; eauto. econs; eauto. econs; eauto. *)
-  (*     inv LOCAL0. ss. clarify. *)
-  (*     erewrite map_write_fence_tview; eauto; cycle 1. *)
-  (*     { eapply read_fence_closed; eauto. inv LCWF. eauto. } *)
-  (*     repeat erewrite map_read_fence. econs; ss; eauto. *)
-  (*     erewrite map_write_fence_sc; eauto. *)
-  (*     + erewrite map_read_fence. auto. *)
-  (*     + eapply read_fence_closed; eauto. inv LCWF. eauto. *)
-  (*   - exists mem_src. esplits; eauto. econs; eauto. econs; eauto. *)
-  (*     econs 2; eauto. econs; eauto. econs; eauto. *)
-  (*     inv LOCAL0. ss. clarify. *)
-  (*     erewrite map_write_fence_tview; eauto; cycle 1. *)
-  (*     { eapply read_fence_closed; eauto. inv LCWF. eauto. } *)
-  (*     repeat erewrite map_read_fence. econs; ss; eauto. *)
-  (*     erewrite map_write_fence_sc; eauto. *)
-  (*     eapply read_fence_closed; eauto. inv LCWF. eauto. *)
-  (*   - exists mem_src. esplits; eauto. econs; eauto. econs; eauto. *)
-  (*     econs 2; eauto. econs; eauto. econs; eauto. econs; eauto. *)
-  (*     ii. ss. erewrite Memory.bot_get in *. clarify. *)
-  (* Qed. *)
+      { eapply mappable_memory_op.
+        - eapply Memory.promise_op; eauto.
+        - eauto.
+        - eauto.
+        - eapply memory_map_mappable; eauto. }
+      i. des. unfold mappable_time in FROM, TO. des.
+      exploit promise_map; eauto. i. des.
+      exists (Local.mk (Local.tview flc0) fprom1). esplits; eauto.
+      + econs; eauto.
+      + econs; eauto. econs; eauto. econs; eauto. econs; eauto.
+        eapply closed_message_map; eauto.
+      + ss. econs; eauto.
+    - inv LCWF. inv STEP0. inv LOCAL0; ss.
+      + esplits; eauto.
+        * econs; eauto.
+        * econs; eauto. econs 2; eauto. econs; eauto.
+      + exploit read_step_map; eauto. i. des.
+        esplits; eauto.
+        * econs; eauto.
+        * econs; eauto. econs 2; eauto. econs; eauto.
+      + unfold mappable_time in SAT. des.
+        hexploit write_step_map; try apply LOCAL1; try eassumption.
+        { econs. }
+        { econs. }
+        { econs. }
+        i. des. esplits; eauto.
+        * econs; eauto.
+        * econs; eauto. econs 2; eauto. econs; eauto.
+      + unfold mappable_time in SAT. des.
+        hexploit read_step_map; try apply LOCAL1; try eassumption. i. des.
+        exploit Local.read_step_future; eauto. i. des.
+        hexploit write_step_map; try apply LOCAL2; try eassumption.
+        { inv READ. ss. }
+        { inv WF2. auto. }
+        i. des. esplits; eauto.
+        * econs; eauto.
+        * econs; eauto. econs 2; eauto. econs; eauto.
+      + hexploit fence_step_map; try apply LOCAL1; try eassumption. i. des.
+        esplits; eauto.
+        * econs; eauto.
+        * econs; eauto. econs 2; eauto. econs; eauto.
+      + hexploit fence_step_map; try apply LOCAL1; try eassumption. i. des.
+        esplits; eauto.
+        * econs; eauto.
+        * econs; eauto. econs 2; eauto. econs; eauto.
+      + inv LOCAL1. esplits; eauto.
+        * econs; eauto.
+        * econs; eauto. econs 2; eauto. econs; eauto.
+          econs; eauto. econs; eauto. inv LOCAL.
+          eapply promise_consistent_mon.
+          { eapply promise_consistent_map; eauto. }
+          { ss. }
+          { refl. }
+  Qed.
 
 End MAPPED.
 
